split the invariant module, but may need a different strategy for the consistency lemma in terms of proof efficiency

paxos-consistency.dfy
@@ -1,10 +1,14 @@
 include "paxos-classic.dfy"
 include "auxiliary.dfy"
+include "paxos-invariants.dfy"
+include "paxos-leader-ballot-invariants.dfy"
 
 module Consistency {
 
     import opened Paxos_protocol
     import opened Auxiliary_lemmas
+    import opened Invariants
+    import opened Leader_ballot_invariants
 
     lemma{:axiom} Quorum()
     ensures |acceptors| == 2 * F + 1
@@ -19,58 +23,6 @@ module Consistency {
         assert |A| + |B| > |acceptors|;
         Intersection(A, B, acceptors);
         a :| a in A && a in B;
-    }
-
-    /** define what a valid state is in a Paxos run
-        we will add invariants into this predicate later
-     */
-    ghost predicate valid(s: TSState) /// the list of invariants for all states
-    requires type_ok(s)
-    {
-        // the followings are the variants that pick up basic features of the Paxos protocol to be used in the proof of the first lemma
-        && (forall c :: c in leaders && (s.leader_decision[c] > 0) ==> (|s.decision_count[c]| >= F+1)) 
-        && (forall c :: c in leaders && (s.leader_decision[c] > 0) ==> (s.leader_propose[c] == s.leader_decision[c]))
-        && (forall c :: c in leaders && s.leader_propose[c] > 0 ==> s.leader_ballot[c] >= 0)
-        && (forall c :: c in leaders ==> s.promise_count[c] <= acceptors)
-        && (forall a, c :: a in acceptors && c in leaders && a in s.promise_count[c] ==> (exists h :: PMsg(s.leader_ballot[c], h, 0) in s.pmsgs[a]))
-        && (forall a :: a in acceptors ==> s.acceptor_state[a].value >= 0)
-//        && (forall a :: a in acceptors ==> !(PMsg(-1, -1, 0) in s.pmsgs[a])) //
-//        && (forall a :: a in acceptors ==> s.acceptor_ballot[a] <= s.acceptor_state[a].highest) //
-//        && (forall a, bn, value :: a in acceptors && CMsg(bn, value) in s.cmsgs[a] ==> bn <= s.acceptor_ballot[a]) //
-//        && (forall a :: a in acceptors && s.acceptor_ballot[a] >= 0 ==> (s.acceptor_state[a].highest >= s.acceptor_ballot[a] && s.acceptor_state[a].value > 0)) //
-
-        // if acceptor a sends a promise to c with a highest confirmed ballot -1, then acceptor a must not have sent confirm message to any leader with a smaller ballot
-        && (forall a, bn, bn', h, value :: a in acceptors && 0 <= bn < bn' && (CMsg(bn, value) in s.cmsgs[a]) ==> 
-               (!(PMsg(bn', h, 0) in s.pmsgs[a])))  //* (1) equivalent to the invariant (2)
-        && (forall a :: a in acceptors ==> (s.acceptor_state[a].value > 0 ==> s.acceptor_state[a].highest >=0) )
-        && (forall a, bn, highest, value :: a in acceptors && (PMsg(bn, highest, value) in s.pmsgs[a]) ==> (highest == -1 ==> value == 0))
-        && (forall a :: a in acceptors && s.acceptor_state[a].value == 0 ==> s.cmsgs[a] == {})
-        && (forall a, bn, highest, value  :: a in acceptors && (PMsg(bn, highest, value) in s.pmsgs[a]) ==> bn <= s.acceptor_state[a].highest)
-        && (forall a, bn, bn', h, value :: a in acceptors && (CMsg(bn, value) in s.cmsgs[a]) && (PMsg(bn', h, 0) in s.pmsgs[a]) ==> bn >= bn') //* (2) equivalent to the invariant (1)
-
-        // a proposed value from c is either from an acceptor, or by c itself if majority promises are collected 
-        // (used for the induction step in the proof of the lemma Min_leader_decision)
-        && (forall c :: c in leaders ==> (s.leader_propose[c] > 0) ==> ( 
-            || |s.promise_count[c]| >= F + 1
-            || exists a, h :: a in acceptors && PMsg(s.leader_ballot[c], h, s.leader_propose[c]) in s.pmsgs[a] // * invariant X
-            ))
-        // if (bn, v) is confirmed, then some leader with bn has proposed v
-        && (forall bn, v, a :: a in acceptors && CMsg(bn, v) in s.cmsgs[a] && v > 0 ==> (exists n :: n in leaders && s.leader_propose[n] == v && s.leader_ballot[n] == bn)) 
-        // the following invariants are required for the induction step in the proof of lemma Min_leader_decision
-        && (forall a :: a in acceptors && s.acceptor_state[a].value > 0 ==> s.acceptor_state[a].highest >= 0)
-        && (forall a :: a in acceptors && s.acceptor_state[a].value > 0 ==> (exists n :: n in leaders && s.leader_propose[n] == s.acceptor_state[a].value && s.leader_ballot[n] <= s.acceptor_state[a].highest))
-        && (forall bn, h, v, a :: a in acceptors && PMsg(bn, h , v) in s.pmsgs[a] && v > 0 ==> 
-           h < bn && (exists n :: n in leaders && 0 <= s.leader_ballot[n] <= h && s.leader_propose[n] == v)) // * invariant Y
-    }
-
-    // the following are invariants used in the proof of lemma Same_ballot_leaders (split from the main body of invariants)
-    ghost predicate valid_leader_ballot(s: TSState) 
-    requires type_ok(s)
-    {
-        && s.ballot >= 0 && s.ballot == |s.ballot_mapping|
-        && (forall c :: c in leaders && s.leader_ballot[c] >= 0 ==> s.leader_ballot[c] < |s.ballot_mapping|)
-        && (forall c :: c in leaders && s.leader_ballot[c] >= 0 ==> s.ballot_mapping[s.leader_ballot[c]] == c)
-        && (forall c1, c2 :: c1 in leaders && c2 in leaders && s.leader_ballot[c1] == s.leader_ballot[c2] > 0 ==> c1 == c2)
     }
 
     lemma Conflict_confirm_promise(s: TSState, c1: Acceptor, c2: Acceptor)
@@ -122,6 +74,7 @@ module Consistency {
     //     if s.leader_ballot[c2] == s.leader_ballot[c1]{
     //         // base case: when c2 == c1, then their proposal should be the same
     //         // assert c1 == c2;
+    //         Same_ballot_leaders(s, c1, c2);
     //     } else { 
     //         // induction step:
     //         //assert s.leader_ballot[c2] > s.leader_ballot[c1];
@@ -133,52 +86,7 @@ module Consistency {
     //     }
     // }
 
-    /** the list of lemmas for all the reachable states and all the transitions, since it's easier to debug in this way.
-     */
-    lemma Inv_init(s: TSState)
-    requires type_ok(s) && init(s)
-    ensures valid(s)
-    {}
-
-    lemma Inv_choose_ballot(s: TSState, s': TSState, c: Acceptor)
-    requires type_ok(s) && type_ok(s') && valid(s) && c in leaders && choose_ballot(s, s', c)
-    ensures valid(s')
-    {}
-
-    lemma Inv_receive_higher_ballot(s: TSState, s': TSState, c: Acceptor, a: Acceptor)
-    requires type_ok(s) && type_ok(s') && valid(s) && c in leaders && a in acceptors && receive_higher_ballot(s, s', c, a)
-    ensures valid(s')
-    {}
-
-    lemma Inv_receive_response_1b(s: TSState, s': TSState, c: Acceptor, a: Acceptor, value: Proposal)
-    requires type_ok(s) && type_ok(s') && valid(s) && c in leaders && a in acceptors && receive_response_1b(s, s', c, a, value)
-    ensures valid(s')
-    {}
-
-    lemma Inv_propose_value_2a(s: TSState, s': TSState, c: Acceptor, value: Proposal)
-    requires  type_ok(s) && type_ok(s') && valid(s) && c in leaders && value != 0 && propose_value_2a(s, s', c, value)
-    ensures valid(s')
-    {}
-
-    lemma Inv_confirm_ballot_2b(s: TSState, s': TSState, c: Acceptor, a: Acceptor, value: Proposal)
-    requires type_ok(s) && type_ok(s') && valid(s) && c in leaders && a in acceptors && value > 0
-    requires confirm_ballot_2b(s, s', c, a, value)
-    ensures valid(s')
-    {}
-
-    lemma Inv_receive_confirm_2b(s: TSState, s': TSState, c: Acceptor, a: Acceptor, bn: int, value: Proposal)
-    requires type_ok(s) && type_ok(s') && valid(s) && c in leaders && a in acceptors && value > 0
-    requires receive_confirm_2b(s, s', c, a, value)
-    ensures valid(s')
-    {}
-
-    lemma Inv_leader_decide(s: TSState, s': TSState, c: Acceptor, value: Proposal)
-    requires type_ok(s) && type_ok(s') && valid(s) && c in leaders && value != 0
-    requires leader_decide(s, s', c, value)
-    ensures valid(s')
-    {}
-
-    lemma consistency(s: TSState, c1: Acceptor, c2: Acceptor)
+    lemma Consistency(s: TSState, c1: Acceptor, c2: Acceptor)
     requires type_ok(s) && valid(s)
     requires c1 in leaders && c2 in leaders && (s.leader_decision[c1] > 0) && (s.leader_decision[c2] > 0)
     //ensures s.leader_decision[c1] == s.leader_decision[c2]
